@prefix owl: <http://www.w3.org/2002/07/owl#>.
@prefix rdfs: <http://www.w3.org/2000/01/rdf-schema#>.
@prefix rdf: <http://www.w3.org/1999/02/22-rdf-syntax-ns#>.

<https://my-model-3u86gh.iri.todo.com/entities/farmer> a owl:Class, rdfs:Class;
    rdfs:label "Farmer"@en;
    rdfs:comment "An individual who engages in the activity of agriculture, growing and harvesting crops."@en.
<https://my-model-3u86gh.iri.todo.com/entities/conducts-planting> a rdf:Property, owl:ObjectProperty;
    rdfs:label "conducts planting"@en;
    rdfs:comment " Indicates which farmer is responsible for a particular planting activity. This association helps attribute specific planting operations to individual farmers, crucial for management and accountability."@en;
    rdfs:domain <https://my-model-3u86gh.iri.todo.com/entities/farmer>;
    rdfs:range <https://my-model-3u86gh.iri.todo.com/entities/planting>.
<https://my-model-3u86gh.iri.todo.com/entities/name> a rdf:Property, owl:DatatypeProperty;
    rdfs:label "name"@en;
    rdfs:comment "The name of the farmer that uniquely identifies the farmer and that is used to refer to the farmer from various documentation, statistical reporting, etc."@en;
    rdfs:domain <https://my-model-3u86gh.iri.todo.com/entities/farmer>.
<https://my-model-3u86gh.iri.todo.com/entities/farms-on> a rdf:Property, owl:ObjectProperty;
    rdfs:label "farms on"@en;
    rdfs:comment "A farmer farms on one or more fields to grow crop on it. Farming includes not only growing crops but also other farming activities such as soil preparation."@en;
    rdfs:domain <https://my-model-3u86gh.iri.todo.com/entities/farmer>;
    rdfs:range <https://my-model-3u86gh.iri.todo.com/entities/field>.
<https://my-model-3u86gh.iri.todo.com/entities/age> a rdf:Property, owl:DatatypeProperty;
    rdfs:label "age"@en;
    rdfs:comment "The age of the farmer in years, used mainly for statistical and reporting purposes."@en;
    rdfs:domain <https://my-model-3u86gh.iri.todo.com/entities/farmer>.
<https://my-model-3u86gh.iri.todo.com/entities/fruit> a owl:Class, rdfs:Class;
    rdfs:label "Fruit"@en;
    rdfs:comment "Plants cultivated for producing their seed-associated fleshy structures that typically are sweet or sour and edible in the raw state, such as apples, bananas, grapes, lemons, oranges, and strawberries."@en;
    rdfs:subClassOf <https://my-model-3u86gh.iri.todo.com/entities/crop>.
<https://my-model-3u86gh.iri.todo.com/entities/vegetable> a owl:Class, rdfs:Class;
    rdfs:label "Vegetable"@en;
    rdfs:comment "Plants cultivated for their parts consumable by humans or other animals as food."@en;
    rdfs:subClassOf <https://my-model-3u86gh.iri.todo.com/entities/crop>.
<https://my-model-3u86gh.iri.todo.com/entities/planting> a owl:Class, rdfs:Class;
    rdfs:label "Planting"@en;
    rdfs:comment "Represents the agricultural activity of planting crops in a specific field during a specific year. It captures the details of the planting process."@en.
<https://my-model-3u86gh.iri.todo.com/entities/results-in-harvest> a rdf:Property, owl:ObjectProperty;
    rdfs:label "results in harvest"@en;
    rdfs:comment "Connects a specific planting activity to the subsequent harvest it produces. This relationship is essential for tracing the agricultural output back to its planting origins, enabling an analysis of the effectiveness of the planting strategies, the impact of environmental conditions, and the overall productivity of agricultural practices."@en;
    rdfs:domain <https://my-model-3u86gh.iri.todo.com/entities/planting>;
    rdfs:range <https://my-model-3u86gh.iri.todo.com/entities/harvest>.
<https://my-model-3u86gh.iri.todo.com/entities/performed-on> a rdf:Property, owl:ObjectProperty;
    rdfs:label "performed on"@en;
    rdfs:comment "Connects the planting activity to the specific field where it occurs, indicating the location of agricultural operations and facilitating field-specific crop management."@en;
    rdfs:domain <https://my-model-3u86gh.iri.todo.com/entities/planting>;
    rdfs:range <https://my-model-3u86gh.iri.todo.com/entities/field>.
<https://my-model-3u86gh.iri.todo.com/entities/involves-crop> a rdf:Property, owl:ObjectProperty;
    rdfs:label "involves crop"@en;
    rdfs:comment "Associates a planting activity with the specific crops being planted. This property is key to understanding the crop variety and its cultivation requirements during the planting process."@en;
    rdfs:domain <https://my-model-3u86gh.iri.todo.com/entities/planting>;
    rdfs:range <https://my-model-3u86gh.iri.todo.com/entities/crop>.
<https://my-model-3u86gh.iri.todo.com/entities/planting-date> a rdf:Property, owl:DatatypeProperty;
    rdfs:label "planting date"@en;
    rdfs:comment " The exact date or period when the crop was planted in the field. This is critical for tracking crop growth stages and scheduling subsequent farming activities."@en;
    rdfs:domain <https://my-model-3u86gh.iri.todo.com/entities/planting>.
<https://my-model-3u86gh.iri.todo.com/entities/planter> a owl:Class, rdfs:Class;
    rdfs:label "Planter"@en;
    rdfs:comment "Machinery designed to plant seeds efficiently and accurately, crucial for optimal crop distribution and growth."@en;
    rdfs:subClassOf <https://my-model-3u86gh.iri.todo.com/entities/machinery>.
<https://my-model-3u86gh.iri.todo.com/entities/crop> a owl:Class, rdfs:Class;
    rdfs:label "Crop"@en;
    rdfs:comment "Plants grown in large amounts and cultivated by farmers for profit or subsistence, including cereals, oil seeds, vegetables, and fruits."@en.
<https://my-model-3u86gh.iri.todo.com/entities/cultivated-variety> a rdf:Property, owl:DatatypeProperty;
    rdfs:label "cultivated variety"@en;
    rdfs:comment "A plant grouping, within a single botanical taxon of the lowest known rank, defined by the reproducible expression of its distinguishing and other genetic characteristics."@en;
    rdfs:domain <https://my-model-3u86gh.iri.todo.com/entities/crop>.
<https://my-model-3u86gh.iri.todo.com/entities/field> a owl:Class, rdfs:Class;
    rdfs:label "Field"@en;
    rdfs:comment "An area of land used for growing crops that can be but does not have to be surrounded by a fence."@en.
<https://my-model-3u86gh.iri.todo.com/entities/irrigation-availability> a rdf:Property, owl:DatatypeProperty;
    rdfs:label "irrigation availability"@en;
    rdfs:comment "Indicates whether the field has access to irrigation systems and the type of irrigation used (e.g., drip, sprinkler, or flood). This is vital for planning water usage and can impact crop selection and planting schedules based on the water needs of the crops."@en;
    rdfs:domain <https://my-model-3u86gh.iri.todo.com/entities/field>.
<https://my-model-3u86gh.iri.todo.com/entities/location> a rdf:Property, owl:DatatypeProperty;
    rdfs:label "location"@en;
    rdfs:comment "Describes the geographical location of the field, which can include specific GPS coordinates or a general description (e.g., near a certain landmark). This helps in locating the field for logistical purposes and for understanding its geographical and climatic context."@en;
    rdfs:domain <https://my-model-3u86gh.iri.todo.com/entities/field>.
<https://my-model-3u86gh.iri.todo.com/entities/soil-ph> a rdf:Property, owl:DatatypeProperty;
    rdfs:label "soil pH"@en;
    rdfs:comment "Indicates the acidity or alkalinity of the soil, which is crucial for managing soil health and fertility. Soil pH can significantly influence crop health and productivity, dictating the types of amendments needed to optimize growing conditions."@en;
    rdfs:domain <https://my-model-3u86gh.iri.todo.com/entities/field>.
<https://my-model-3u86gh.iri.todo.com/entities/size> a rdf:Property, owl:DatatypeProperty;
    rdfs:label "size"@en;
    rdfs:comment "Measures the total area of the field, typically expressed in hectares. This attribute is fundamental for planning the distribution of crops, determining the amount of seeds needed, and calculating the expected yield."@en;
    rdfs:domain <https://my-model-3u86gh.iri.todo.com/entities/field>.
<https://my-model-3u86gh.iri.todo.com/entities/soil-type> a rdf:Property, owl:DatatypeProperty;
    rdfs:label "soil type"@en;
    rdfs:comment "Specifies the type of soil present in the field, such as loamy, sandy, clay, or silt. Soil type affects water retention, nutrient availability, and the types of crops that can be successfully cultivated."@en;
    rdfs:domain <https://my-model-3u86gh.iri.todo.com/entities/field>.
<https://my-model-3u86gh.iri.todo.com/entities/topography> a rdf:Property, owl:DatatypeProperty;
    rdfs:label "topography"@en;
    rdfs:comment "Describes the physical layout of the land, including its flatness, slope, and elevation. Topography influences water drainage, erosion risk, and the suitability of various agricultural machinery."@en;
    rdfs:domain <https://my-model-3u86gh.iri.todo.com/entities/field>.
<https://my-model-3u86gh.iri.todo.com/entities/harvest> a owl:Class, rdfs:Class;
    rdfs:label "Harvest"@en;
    rdfs:comment "The production that is obtained from crops. It is quantified and evaluated in terms of quantity and quality. It represents the final output of the agricultural cycle."@en.
<https://my-model-3u86gh.iri.todo.com/entities/quantity> a rdf:Property, owl:DatatypeProperty;
    rdfs:label "quantity"@en;
    rdfs:comment "The total quantity of the harvest, measured in kilograms. This attribute is crucial for determining the productivity and success of the crop."@en;
    rdfs:domain <https://my-model-3u86gh.iri.todo.com/entities/harvest>.
<https://my-model-3u86gh.iri.todo.com/entities/harvest-date> a rdf:Property, owl:DatatypeProperty;
    rdfs:label "harvest date"@en;
    rdfs:comment "The specific date or time period when the harvest was collected. Timing is crucial for maximizing yield and ensuring the best quality of the harvested product"@en;
    rdfs:domain <https://my-model-3u86gh.iri.todo.com/entities/harvest>.
<https://my-model-3u86gh.iri.todo.com/entities/quality> a rdf:Property, owl:DatatypeProperty;
    rdfs:label "quality"@en;
    rdfs:comment ": The quality of the harvest, which may include factors like size, ripeness, nutritional value, and absence of pests or diseases. High-quality harvests are crucial for market acceptance and consumer satisfaction."@en;
    rdfs:domain <https://my-model-3u86gh.iri.todo.com/entities/harvest>.
<https://my-model-3u86gh.iri.todo.com/entities/harvested-by> a rdf:Property, owl:ObjectProperty;
    rdfs:label "harvested by"@en;
    rdfs:comment "Connects the harvested produce to the farmer who performed the harvest and who is also responsible for evaluating the quality and quantity of the harvested crop, essential for market transactions and crop performance analysis."@en;
    rdfs:domain <https://my-model-3u86gh.iri.todo.com/entities/harvest>;
    rdfs:range <https://my-model-3u86gh.iri.todo.com/entities/farmer>.
<https://my-model-3u86gh.iri.todo.com/entities/tractor> a owl:Class, rdfs:Class;
    rdfs:label "Tractor"@en;
    rdfs:comment "Versatile piece of machinery essential for multiple farming tasks, from soil preparation to crop maintenance."@en;
    rdfs:subClassOf <https://my-model-3u86gh.iri.todo.com/entities/machinery>.
<https://my-model-3u86gh.iri.todo.com/entities/seed-plant> a owl:Class, rdfs:Class;
    rdfs:label "Seed Plant"@en;
    rdfs:comment "Plants grown for oil production from seeds, like sunflower and soybean, significant for both food and industrial uses."@en;
    rdfs:subClassOf <https://my-model-3u86gh.iri.todo.com/entities/crop>.
<https://my-model-3u86gh.iri.todo.com/entities/cereal> a owl:Class, rdfs:Class;
    rdfs:label "Cereal"@en;
    rdfs:comment "A cereal is a plant cultivated for its edible grain."@en;
    rdfs:subClassOf <https://my-model-3u86gh.iri.todo.com/entities/crop>.
<https://my-model-3u86gh.iri.todo.com/entities/machinery> a owl:Class, rdfs:Class;
    rdfs:label "Machinery"@en;
    rdfs:comment "Mechanical tools and equipment used in farming, crucial for tasks such as plowing, seeding, spraying, and harvesting."@en.
<https://my-model-3u86gh.iri.todo.com/entities/used-for-field-preparation> a rdf:Property, owl:ObjectProperty;
    rdfs:label "used for field preparation"@en;
    rdfs:comment "Indicates that certain types of machinery, such as tractors equipped with specific attachments, are used to prepare the field for planting. This process might include plowing, tilling, and conditioning the soil to create an optimal planting environment."@en;
    rdfs:domain <https://my-model-3u86gh.iri.todo.com/entities/machinery>;
    rdfs:range <https://my-model-3u86gh.iri.todo.com/entities/planting>.
<https://my-model-3u86gh.iri.todo.com/entities/year-of-manufacturing> a rdf:Property, owl:DatatypeProperty;
    rdfs:label "year of manufacturing"@en;
    rdfs:comment "The year the machinery was manufactured, indicating its age and potential modernity in technology."@en;
    rdfs:domain <https://my-model-3u86gh.iri.todo.com/entities/machinery>.
<https://my-model-3u86gh.iri.todo.com/entities/model> a rdf:Property, owl:DatatypeProperty;
    rdfs:label "model"@en;
    rdfs:comment "Identifies the model of the machinery, which affects its functionality and suitability for specific tasks."@en;
    rdfs:domain <https://my-model-3u86gh.iri.todo.com/entities/machinery>.
<https://my-model-3u86gh.iri.todo.com/entities/used-for-planting> a rdf:Property, owl:ObjectProperty;
    rdfs:label "used for planting"@en;
    rdfs:comment " Indicates that a specific piece of machinery is employed in the planting process. This property links machinery like planters and some types of tractors that are specifically outfitted for or used during the planting of crops."@en;
    rdfs:domain <https://my-model-3u86gh.iri.todo.com/entities/machinery>;
    rdfs:range <https://my-model-3u86gh.iri.todo.com/entities/planting>.
<https://my-model-3u86gh.iri.todo.com/entities/used-for-harvesting> a rdf:Property, owl:ObjectProperty;
    rdfs:label "used for harvesting"@en;
    rdfs:comment "Connects a piece of machinery to its use in the harvesting process. This association is specific to machinery like combines, harvesters, and other equipment that is primarily utilized to collect and process crops at the end of their growing cycle."@en;
    rdfs:domain <https://my-model-3u86gh.iri.todo.com/entities/machinery>;
    rdfs:range <https://my-model-3u86gh.iri.todo.com/entities/harvest>.
<https://my-model-3u86gh.iri.todo.com/entities/harvester> a owl:Class, rdfs:Class;
    rdfs:label "Harvester"@en;
    rdfs:comment "Specialized machinery that is used for harvesting. It also includes machinery that combines harvesting tasks such as reaping, threshing, and winnowing into a single operation."@en;
    rdfs:subClassOf <https://my-model-3u86gh.iri.todo.com/entities/machinery>.
<https://my-model-3u86gh.iri.todo.com/entities/sprayer> a owl:Class, rdfs:Class;
    rdfs:label "Sprayer"@en;
    rdfs:comment "Used for the precise application of liquids like pesticides and fertilizers, vital for crop protection and growth enhancement."@en;
    rdfs:subClassOf <https://my-model-3u86gh.iri.todo.com/entities/machinery>.
