@prefix owl: <http://www.w3.org/2002/07/owl#>.
@prefix rdfs: <http://www.w3.org/2000/01/rdf-schema#>.
@prefix rdf: <http://www.w3.org/1999/02/22-rdf-syntax-ns#>.

<department> a owl:Class, rdfs:Class;
    rdfs:label "Department"@en;
    rdfs:comment "A department of a company, e.g., accounting, marketing, or any other department."@en.
<title> a rdf:Property, owl:DatatypeProperty;
    rdfs:label "title"@en;
    rdfs:comment "The title of the department."@en;
    rdfs:domain <department>.
<manager> a owl:Class, rdfs:Class;
    rdfs:label "Manager"@en;
    rdfs:comment "A manager is an employ that still does much of what other employees do, but they also have extra responsibilities depending on their level in the company hierarchy. The managers helps keep things running smoothly and make sure departments they manage are productive."@en;
    rdfs:subClassOf <employee>.
<manages> a rdf:Property, owl:ObjectProperty;
    rdfs:label "manages"@en;
    rdfs:comment "Determines the department whose productivity the manager ensures."@en;
    rdfs:domain <manager>;
    rdfs:range <department>.
<level> a rdf:Property, owl:DatatypeProperty;
    rdfs:label "level"@en;
    rdfs:comment "The level of the manager in the company hierarchy."@en;
    rdfs:domain <manager>.
<employee> a owl:Class, rdfs:Class;
    rdfs:label "Employee"@en;
    rdfs:comment "An employee of a company."@en.
<personal-number> a rdf:Property, owl:DatatypeProperty;
    rdfs:label "personal number"@en;
    rdfs:comment "The personal number that uniquely identifies the employee in the company."@en;
    rdfs:domain <employee>.
<works-in> a rdf:Property, owl:ObjectProperty;
    rdfs:label "works in"@en;
    rdfs:comment "An employee works in just one department, which is a part of how the company organizes its work."@en;
    rdfs:domain <employee>;
    rdfs:range <department>.
<name> a rdf:Property, owl:DatatypeProperty;
    rdfs:label "name"@en;
    rdfs:comment "The name that other employees in the company use to address the employee."@en;
    rdfs:domain <employee>.
<role> a rdf:Property, owl:DatatypeProperty;
    rdfs:label "role"@en;
    rdfs:comment "The specific role of the employee"@en;
    rdfs:domain <employee>.
<contact-email> a rdf:Property, owl:DatatypeProperty;
    rdfs:label "contact email"@en;
    rdfs:comment "An email address essential for remote contact with the employee."@en;
    rdfs:domain <employee>.
